lib_misc/PtrdiffWrapper.fsti
@@ -3,16 +3,21 @@ module PtrdiffWrapper
 module U32 = FStar.UInt32
 module US = FStar.SizeT
 module UP = FStar.PtrdiffT
+module U64 = FStar.UInt64
 
 open FStar.Mul
 open Config
 
 // conservative axiomatization, C23 changed guarantees about ptrdiff_t bit width
-// this is an assume val
-val ptrdiff_max: v:UP.t{
-  UP.v v >= pow2 16 - 1 /\
-  (exists (k:nat). UP.v v = pow2 k - 1)
-}
+//TODO: add const qualifier/upstream it to FStar.PtrdiffT
+//assume val ptrdiff_max: v:UP.t{
+//  UP.v v >= pow2 16 - 1 /\
+//  (exists (k:nat). UP.v v = pow2 k - 1)
+//}
+
+//TODO: remove this hardcoded constant
+//currently equal to (PTRDIFF_MAX/2)+1,
+//that is, 2^62 on x86_64-Linux
 
 open MiscArith
 
@@ -22,19 +27,117 @@ let mmap_bound : v:US.t{
   US.v v % U32.v page_size = 0
 }
   =
-  let ptrdiff_max_as_sizet = UP.ptrdifft_to_sizet ptrdiff_max in
-  // US.fits(x) where x = 2^n-1
-  // y = x/2 = (2^n-1)/2 = 2^{n-1}-1
-  let r = US.add (US.div ptrdiff_max_as_sizet 2sz) 1sz in
-  eliminate exists (k:nat). UP.v ptrdiff_max = pow2 k - 1
-    returns (US.v r % U32.v page_size = 0)
-    with _. (
-      assert (UP.v ptrdiff_max == pow2 k - 1);
-      assert (US.v r == pow2 (k-1));
-      assert (U32.v page_size == pow2 12);
-      pow2_is_increasing 12 (k-1);
-      pow2_mod 12 (k-1);
-      ()
-  );
-  r
-  //normalize_term r
+  [@inline_let] let x = pow2 62 in
+  assume (US.fits x);
+  assume (US.fits (x + 2));
+  assume (US.fits (x + U32.v page_size));
+  pow2_mod 12 62;
+  normalize_term (US.uint_to_t x)
+
+//let mmap_bound : v:US.t{
+//  US.fits (US.v v + 2) /\
+//  US.fits (US.v v + U32.v page_size) /\
+//  US.v v % U32.v page_size = 0
+//}
+//  =
+//  let ptrdiff_max_as_sizet = UP.ptrdifft_to_sizet ptrdiff_max in
+//  // US.fits(x) where x = 2^n-1
+//  // y = x/2 = (2^n-1)/2 = 2^{n-1}-1
+//  let r = US.add (US.div ptrdiff_max_as_sizet 2sz) 1sz in
+//  eliminate exists (k:nat). UP.v ptrdiff_max = pow2 k - 1
+//    returns (US.v r % U32.v page_size = 0)
+//    with _. (
+//      assert (UP.v ptrdiff_max == pow2 k - 1);
+//      assert (US.v r == pow2 (k-1));
+//      assert (U32.v page_size == pow2 12);
+//      pow2_is_increasing 12 (k-1);
+//      pow2_mod 12 (k-1);
+//      ()
+//  );
+//  r
+
+module FML = FStar.Math.Lemmas
+
+#push-options "--fuel 0 --ifuel 0 --z3rlimit 100"
+noextract
+let nearest_multiple_upper_rounding
+  (n: nat)
+  (multiple: nat{multiple > 0})
+  : Pure nat
+  (requires True)
+  (ensures fun r ->
+    r >= 0 /\
+    r % multiple == 0 /\
+    r >= n /\
+    r - n < multiple
+  )
+  =
+  if n % multiple <> 0
+  then (
+    let r = n - (n % multiple) + multiple in
+    FML.euclidean_division_definition n multiple;
+    assert (n - (n % multiple) == (n/multiple)*multiple);
+    lemma_mod_mul2 (n/multiple) multiple multiple;
+    assert ((n - (n % multiple)) % multiple == 0);
+    lemma_mod_plus2 (n - (n % multiple)) multiple multiple;
+    r
+  ) else n
+
+let rec nearest_multiple_upper_rounding_lemma
+  (n: nat)
+  (multiple: nat{multiple > 0})
+  (k: nat)
+  : Lemma
+  (requires k >= n /\ k % multiple == 0)
+  (ensures
+    k >= nearest_multiple_upper_rounding n multiple
+  )
+  (decreases k)
+  =
+  let n' = nearest_multiple_upper_rounding n multiple in
+  assert (n' >= n /\ n' % multiple == 0);
+  if k < n'
+  then (
+    assert (n' > n);
+    assert (n % multiple <> 0);
+    let diff = n' - k in
+    assert (0 < diff);
+    assert (n' % multiple == 0);
+    assert (k % multiple == 0);
+    lemma_mod_add_inv k multiple;
+    assert ((-k) % multiple == 0);
+    lemma_mod_plus2 (-k) n' multiple;
+    assert (diff % multiple == 0);
+    assert (diff >= multiple);
+    if diff >= multiple
+    then nearest_multiple_upper_rounding_lemma n multiple (k - multiple)
+    else ()
+ ) else ()
+
+noextract
+let spec_mmap_actual_size (size: nat)
+  : Pure nat
+  (requires True)
+  (ensures fun r ->
+    r >= 0 /\
+    r % (U32.v page_size) == 0 /\
+    r >= size /\
+    r - size < (U32.v page_size)
+  )
+  =
+  nearest_multiple_upper_rounding size (U32.v page_size)
+
+let mmap_actual_size (size: US.t)
+  : Pure US.t
+  (requires
+    US.fits (US.v size + U32.v page_size)
+  )
+  (ensures fun r ->
+    US.v r == spec_mmap_actual_size (US.v size)
+  )
+  =
+  let rem = US.rem size (u32_to_sz page_size) in
+  if rem <> 0sz
+  then US.add (US.sub size rem) (u32_to_sz page_size)
+  else size
+#pop-options
