src/LargeAlloc.fst
@@ -256,7 +256,8 @@ let find = Map.M.find
 
 open Config
 
-let mmap_actual_size = Mman.mmap_actual_size
+inline_for_extraction noextract
+let mmap_actual_size = PtrdiffWrapper.mmap_actual_size
 
 #push-options "--fuel 1 --ifuel 1 --z3rlimit 100"
 [@@ __steel_reduce__]
